LynxTest.lean
@@ -12,3 +12,4 @@ import LynxTest.Tactic.Pure
 import LynxTest.Tactic.Failures
 import LynxTest.Modules.Erlang
 import LynxTest.Modules.Maps
+import LynxTest.Modules.Process
